Próba ratowania koinduktywnego mnożenia, nie do końca udana.

book/F2.v
@@ -1455,6 +1455,103 @@ Definition sub' : Type :=
     forall n m r : conat, f n m = r -> Sub n m r}.
 (* end hide *)
 
+(** * Dupa konia w polewie ogórkowej *)
+
+Inductive sim2_aux (n m : conat) (S : conat -> conat -> Prop) : Prop :=
+    | sim2_aux_zero :
+        pred n = None -> pred m = None -> sim2_aux n m S
+    | sim2_aux_succ :
+        forall
+          (n' : conat) (Hn : S n (succ n'))
+          (m' : conat) (Hm : S m (succ m'))
+          (Hsim2 : S n' m'),
+            sim2_aux n m S.
+
+Hint Constructors sim2_aux : core.
+
+CoInductive sim2 (n m : conat) : Prop :=
+{
+    sim2' : sim2_aux n m sim2;
+}.
+
+Hint Constructors sim2 : core.
+
+Require Import Coq.Classes.RelationClasses.
+
+Instance sim2_refl :
+  Reflexive sim2.
+(* begin hide *)
+Proof.
+  red.
+  cofix CH.
+  constructor.
+  destruct x as [[]]; eauto.
+Qed.
+(* end hide *)
+
+Instance sim2_symm :
+  Symmetric sim2.
+(* begin hide *)
+Proof.
+  red.
+  cofix CH.
+  destruct 1 as [[]]; constructor; eauto.
+Qed.
+(* end hide *)
+
+Instance sim2_trans :
+  Transitive sim2.
+(* begin hide *)
+Proof.
+  red.
+  cofix CH.
+  destruct 1 as [[]], 1 as [[]]; constructor; eauto.
+Qed.
+(* end hide *)
+
+Hint Resolve sim_refl sim_sym : core.
+
+Lemma sim_sim2 :
+  forall n m : conat,
+    sim n m -> sim2 n m.
+(* begin hide *)
+Proof.
+  cofix CH.
+  destruct 1 as [[[H1 H2] | (n' & m' & H1 & H2 & H3)]];
+  constructor.
+    eauto.
+    eright.
+      Focus 3. apply CH. eassumption.
+      apply CH; constructor; right; cbn. exists n', n'. repeat (split; trivial).
+      apply CH; constructor; right; cbn. exists m', m'. repeat (split; trivial).
+Qed.
+(* end hide *)
+
+Lemma sim2_add_zero_l :
+  forall n m : conat,
+    pred n = None -> sim2 (add n m) m.
+(* begin hide *)
+Proof.
+  intros n **.
+  constructor. destruct (pred m) eqn: Heq.
+    Focus 2. left; cbn; rewrite ?H; assumption.
+    eright.
+Admitted.
+(* end hide *)
+
+Lemma sim2_add :
+  forall n1 n2 m1 m2 : conat,
+    sim2 n1 n2 -> sim2 m1 m2 -> sim2 (add n1 m1) (add n2 m2).
+(* begin hide *)
+Proof.
+  cofix CH.
+  intros n1 n2 m1 m2.
+  destruct 1 as [[Hn1 Hn2 | n1' Hn1 n2' Hn2]].
+    intro. rewrite !sim2_add_zero_l; assumption.
+    constructor. eright.
+Admitted.
+(* end hide *)
+
 (** * Mnożenie (TODO) *)
 
 Inductive Mul_aux (n m r : conat) (M : conat -> conat -> conat -> Prop) : Prop :=
@@ -1466,9 +1563,8 @@ Inductive Mul_aux (n m r : conat) (M : conat -> conat -> conat -> Prop) : Prop :
         forall
           (n' : conat) (Hn : pred n = Some n')
           (m' : conat) (Hm : pred m = Some m')
-          (r' : conat) (Hr : pred r = Some r')
-          (HMul : M n' m' r')
-          (Hsim : sim r (succ (add n' (add m' r')))), Mul_aux n m r M.
+          (r' : conat) (Hsim : sim2 r (succ (add n' (add m' r'))))
+          (HMul : M n' m' r'), Mul_aux n m r M.
 
 Hint Constructors Mul_aux : coind.
 
@@ -1501,54 +1597,54 @@ Proof.
 Qed.
 (* end hide *)
 
-Lemma Mul_one_l :
-  forall n r : conat, Mul (succ zero) n r -> sim n r.
-(* begin hide *)
-Proof.
-  destruct 1 as [[]];
-  constructor; cbn in *.
-    congruence.
-    left. split; assumption.
-    right. do 2 eexists. do 2 (split; try eassumption).
-      inv Hn. destruct HMul. inv Mul'0; cbn in *; subst.
-        admit.
-        admit.
-        congruence.
-Admitted.
-(* end hide *)
-
-Lemma Mul_one_r :
-  forall n r : conat, Mul n (succ zero) r -> sim n r.
-(* begin hide *)
-Proof.
-  destruct 1 as [[]];
-  constructor; cbn in *.
-    left. split; assumption.
-    congruence.
-    right. do 2 eexists. do 2 (split; try eassumption).
-      inv Hm. destruct HMul. inv Mul'0; cbn in *; subst.
-        admit.
-        admit.
-        congruence.
-Admitted.
-(* end hide *)
-
 Lemma Mul_det :
   forall n m r1 r2 : conat,
-    Mul n m r1 -> Mul n m r2 -> sim r1 r2.
+    Mul n m r1 -> Mul n m r2 -> sim2 r1 r2.
 (* begin hide *)
 Proof.
   cofix CH.
   do 2 destruct 1 as [[]];
   try congruence.
-  1-4: constructor; eauto.
-  constructor. right. do 2 eexists. split.
-    exact Hr.
-    split.
-      exact Hr0.
-      rewrite Hn in Hn0. inv Hn0. rewrite Hm in Hm0. inv Hm0.
-        eapply CH; eassumption.
+    1-4: constructor; eauto.
+    constructor. eright.
+      eassumption.
+      eassumption.
+      {
+        rewrite Hn in Hn0. inv Hn0.
+        rewrite Hm in Hm0. inv Hm0.
+        eapply CH.
+        repeat apply sim2_add.
+Admitted.
+(* end hide *)
+
+Lemma sim2_succ :
+  forall n m : conat,
+    sim2 n m -> sim2 (succ n) (succ m).
+(* begin hide *)
+Proof.
+  constructor. eright.
+    reflexivity.
+    reflexivity.
+    assumption.
 Qed.
+(* end hide *)
+
+Lemma sim2_add_assoc :
+  forall a b c : conat,
+    sim2 (add a (add b c)) (add (add a b) c).
+(* begin hide *)
+Proof.
+
+Admitted.
+(* end hide *)
+
+Lemma sim2_add_comm :
+  forall n m : conat,
+    sim2 (add n m) (add m n).
+(* begin hide *)
+Proof.
+
+Admitted.
 (* end hide *)
 
 Lemma Mul_comm :
@@ -1561,37 +1657,101 @@ Proof.
     constructor 2; assumption.
     constructor 1; assumption.
     econstructor 3; try eassumption.
+      {
+        rewrite Hsim.
+        apply sim2_succ.
+        setoid_rewrite sim2_add_assoc.
+        apply sim2_add.
+          apply sim2_add_comm.
+          reflexivity.
+      }
       apply CH. assumption.
-      rewrite Hsim. apply sim_succ. rewrite <- !add_assoc. apply sim_add.
-        apply add_comm.
-        apply sim_refl.
 Qed.
 (* end hide *)
 
-Hint Constructors sim : coind.
+Hint Constructors sim sim2 : coind.
+
+Definition osim (on om : option conat) : Prop :=
+match on, om with
+    | Some n, Some m => sim2 n m
+    | None  , None   => True
+    | _     , _      => False
+end.
+
+Lemma sim2_pred :
+  forall n m : conat,
+    sim2 n m -> osim (pred n) (pred m).
+(* begin hide *)
+Proof.
+  intros n m [[-> -> | ]].
+    cbn. trivial.
+    destruct n as [[]], m as [[]]; cbn; trivial.
+      inv Hn. inv sim2'0; cbn in *.
+        congruence.
+        inv Hm. inv sim2'0; cbn in *.
+          congruence.
+          admit.
+      admit.
+      admit.
+Admitted.
+(* end hide *)
 
 Lemma Mul_assoc :
   forall {a b c r1 r2 s1 s2 : conat},
     Mul a b r1 -> Mul r1 c r2 ->
     Mul b c s1 -> Mul a s1 s2 ->
-      sim r2 s2.
+      sim2 r2 s2.
 (* begin hide *)
 Proof.
   cofix CH.
   do 4 (destruct 1 as [[]]);
-  try congruence; auto with coind.
-  constructor.
-    right. do 2 eexists. split.
+  try congruence; auto with coind;
+  repeat match goal with
+      | H1 : pred ?a = Some _, H2 : pred ?a = Some _ |- _ =>
+          rewrite H1 in H2; inv H2
+  end.
+    apply sim2_pred in Hsim. rewrite Hn0 in Hsim. cbn in Hsim. contradiction.
+    apply sim2_pred in Hsim1. rewrite Hm2 in Hsim1. cbn in Hsim1. contradiction.
+    constructor. eright.
       eassumption.
-      split.
-        eassumption.
-        {
-          repeat match goal with
-              | H1 : pred ?a = Some _, H2 : pred ?a = Some _ |- _ =>
-                  rewrite H1 in H2; inv H2
-          end.
-          eapply (CH _ _ _ _ _ _ _ HMul HMul0 HMul1 HMul2).
-        }
+      eassumption.
+      repeat apply sim2_add.
+Admitted.
+(* end hide *)
+
+Lemma sim_add_zero :
+  forall n m : conat,
+    sim (add n m) zero -> sim n zero /\ sim m zero.
+(* begin hide *)
+Proof.
+  split; destruct H as [[[] | ]]; constructor.
+    left. cbn in H. destruct (pred n); inv H.
+    decompose [ex and] H; cbn in *; congruence.
+    left. cbn in H. destruct (pred n); inv H.
+    decompose [ex and] H; cbn in *; congruence.
+Qed.
+(* end hide *)
+
+Lemma Mul_one_l :
+  forall n r : conat, Mul (succ zero) n r -> sim n r.
+(* begin hide *)
+Proof.
+  destruct 1 as [[]].
+    constructor. cbn in Hn. congruence.
+    constructor. left. split; assumption.
+    inv Hn. apply Mul_zero_l in HMul. assert (sim r (succ r')).
+      constructor. cbn. right. do 2 eexists. do 2 (split; eauto). reflexivity.
+      rewrite H in Hsim. apply sim_succ_inv in Hsim. rewrite HMul in Hsim at 1.
+        symmetry in Hsim. rewrite add_zero_l in Hsim. apply sim_add_zero in Hsim. destruct Hsim.
+        constructor. right. do 2 eexists. do 2 (split; eauto). rewrite H0, H1. reflexivity.
+Qed.
+(* end hide *)
+
+Lemma Mul_one_r :
+  forall n r : conat, Mul n (succ zero) r -> sim n r.
+(* begin hide *)
+Proof.
+  intros. apply Mul_comm in H. apply Mul_one_l. assumption.
 Qed.
 (* end hide *)
 
@@ -1617,13 +1777,53 @@ end.
 
 Compute from_conat 10 (mul' (succ (succ zero)) (succ (succ zero)) zero).
 
+Lemma mul'_zero_l :
+  forall c acc : conat,
+    mul' zero c acc = acc.
+(* begin hide *)
+Proof.
+  intros. apply eq_pred. cbn. reflexivity.
+Qed.
+(* end hide *)
+
+Lemma mul'_zero_r :
+  forall n m acc : conat,
+    pred m = None -> mul' n m acc = acc.
+(* begin hide *)
+Proof.
+  intros. apply eq_pred. cbn. rewrite H. destruct (pred n); reflexivity.
+Qed.
+(* end hide *)
+
 Lemma Mul_mul' :
   forall n m r acc : conat,
-    Mul n m r -> sim (mul' n m acc) (add acc r).
+    Mul n m r -> sim (mul' n m acc) (add r acc).
 (* begin hide *)
 Proof.
   cofix CH.
-  destruct 1 as [[]];
+  destruct 1 as [[]].
+    replace n with zero.
+      rewrite mul'_zero_l. replace r with zero.
+        rewrite add_zero_l. reflexivity.
+        apply eq_pred. cbn. congruence.
+      apply eq_pred. cbn. congruence.
+    rewrite mul'_zero_r.
+      replace r with zero.
+        rewrite add_zero_l. reflexivity.
+        apply eq_pred. cbn. congruence.
+      assumption.
+    constructor. right. eexists. exists (add r' acc). split.
+      cbn. rewrite Hn, Hm. reflexivity.
+      split.
+        cbn. rewrite Hr. reflexivity.
+        {
+          specialize (CH _ _ _ (add n' (add m' acc)) HMul).
+          rewrite CH. apply sim_add. Guarded.
+            reflexivity.
+          
+
+
+
   destruct acc as [[acc' |]];
   cbn.
     constructor; cbn. right. exists acc', (add acc' r). rewrite Hn. split.
@@ -1643,6 +1843,12 @@ Proof.
           apply eq_pred. cbn. congruence.
     constructor; cbn. rewrite Hm. left. destruct (pred n); split; trivial.
     constructor; cbn. rewrite Hn, Hm. right. do 2 eexists. do 2 (split; try reflexivity).
+      eapply sim_trans.
+        apply CH. eassumption.
+        rewrite !add_assoc. Check add_succ_r.
+      rewrite CH.
+        2: eassumption. Guarded.
+        rewrite Hsim.
       admit.
     constructor; cbn. rewrite Hn, Hm. right. do 2 eexists. split.
       reflexivity.
